code/experimental/salsa-family/Hacl.Impl.Chacha20.Vec128.State.fst
@@ -1,0 +1,195 @@
+module Hacl.Impl.Chacha20.Vec128.State
+
+open FStar.Mul
+open FStar.HyperStack
+open FStar.ST
+open FStar.Buffer
+open Hacl.Cast
+open Hacl.Spec.Endianness
+open Hacl.Endianness
+open Spec.Chacha20_vec
+open C.Loops
+
+module Spec = Spec.Chacha20
+module U32 = FStar.UInt32
+module H8  = Hacl.UInt8
+module H32 = Hacl.UInt32
+open Hacl.UInt32x4
+
+let u32 = U32.t
+let h32 = H32.t
+let uint8_p = buffer H8.t
+
+type state = b:Buffer.buffer vec{length b = 4}
+let blocks = U32.(vec_size /^ 4ul)
+let vecsizebytes = U32.(vec_size *^ 4ul)
+
+#reset-options "--max_fuel 0 --z3rlimit 100"
+
+[@ "c_inline"]
+val state_alloc:
+  unit ->
+  StackInline state
+    (requires (fun h -> True))
+    (ensures (fun h0 st h1 -> (st `unused_in` h0) /\ live h1 st /\ modifies_0 h0 h1 /\ frameOf st == h1.tip
+      /\ Map.domain h1.h == Map.domain h0.h))
+[@ "c_inline"]
+let state_alloc () =
+  create zero 4ul
+
+
+[@ "c_inline"]
+val state_incr:
+    k:state ->
+    Stack unit
+      (requires (fun h -> live h k))
+      (ensures  (fun h0 _ h1 -> live h1 k /\ modifies_1 k h0 h1 /\ live h0 k /\
+        (let st0 = as_seq h0 k in
+         let st1 = as_seq h1 k in
+         st1 == Seq.upd st0 3 (Spec.Chacha20_vec.op_Plus_Percent_Hat (Seq.index st0 3) one_le))))
+[@ "c_inline"]
+let state_incr k =
+    let k3 = k.(3ul) in
+    k.(3ul) <- vec_add k3 one_le
+
+[@ "c_inline"]
+val state_to_key:
+    k:state ->
+    Stack unit
+      (requires (fun h -> live h k))
+      (ensures  (fun h0 _ h1 -> h0 == h1))
+[@ "c_inline"]
+let state_to_key k = ()
+
+
+[@ "c_inline"]
+val state_to_key_block:
+    stream_block:uint8_p{length stream_block = 64 * U32.v blocks} ->
+    k:state{disjoint k stream_block} ->
+    Stack unit
+      (requires (fun h -> live h k))
+      (ensures  (fun h0 _ h1 -> live h0 k /\ modifies_1 k h0 h1 /\ live h1 stream_block /\
+        (let stream_block = as_seq h1 stream_block in
+         let k = as_seq h0 k in
+         let op_String_Access = Seq.index in
+         stream_block == FStar.Seq.(Spec.Lib.uint32s_to_le 4 (vec_as_seq k.[0]) @|
+                                    Spec.Lib.uint32s_to_le 4 (vec_as_seq k.[1]) @|
+                                    Spec.Lib.uint32s_to_le 4 (vec_as_seq k.[2]) @|
+                                    Spec.Lib.uint32s_to_le 4 (vec_as_seq k.[3])))))
+[@ "c_inline"]
+let state_to_key_block stream_block k =
+  admit();
+  state_to_key k;
+  let bb = U32.(blocks *^ 16ul) in
+  let bb2 = U32.(bb *^ 2ul) in
+  let bb3 = U32.(bb *^ 3ul) in
+  let k0 = k.(0ul) in
+  let k1 = k.(1ul) in
+  let k2 = k.(2ul) in
+  let k3 = k.(3ul) in
+  vec_store_le (Buffer.sub stream_block 0ul bb) k.(0ul);
+  vec_store_le (Buffer.sub stream_block bb  16ul) k.(1ul);
+  vec_store_le (Buffer.sub stream_block bb2 16ul) k.(2ul);
+  vec_store_le (Buffer.sub stream_block bb3 16ul) k.(3ul)
+
+
+[@ "substitute"]
+val constant_setup_:
+  c:state ->
+  Stack unit
+    (requires (fun h -> live h c))
+    (ensures  (fun h0 _ h1 -> live h1 c /\ modifies_1 c h0 h1 /\ live h0 c /\
+      (let st0 = as_seq h0 c in let st1 = as_seq h1 c in let op_String_Access = Seq.index in
+       let open Spec.Chacha20_vec in let open FStar.Seq in
+       st1.[0] == Seq.Create.create_4 c0 c1 c2 c3 /\
+       st0.[1] == st1.[1] /\ st0.[2] == st1.[2] /\ st0.[3] == st1.[3])))
+[@ "substitute"]
+let constant_setup_ st =
+  st.(0ul)  <- vec_load_32x4 (uint32_to_sint32 0x61707865ul)
+  	       		     (uint32_to_sint32 0x3320646eul)
+			     (uint32_to_sint32 0x79622d32ul)
+			     (uint32_to_sint32 0x6b206574ul)
+
+
+[@ "substitute"]
+val constant_setup:
+  c:state ->
+  Stack unit
+    (requires (fun h -> live h c))
+    (ensures  (fun h0 _ h1 -> live h1 c /\ modifies_1 c h0 h1 /\ live h0 c /\
+      (let st0 = as_seq h0 c in let st1 = as_seq h1 c in let op_String_Access = Seq.index in
+       let open Spec.Chacha20_vec in let open FStar.Seq in
+       st1.[0] == Seq.Create.create_4 c0 c1 c2 c3 /\
+       st0.[1] == st1.[1] /\ st0.[2] == st1.[2] /\ st0.[3] == st1.[3])))
+[@ "substitute"]
+let constant_setup st =
+  constant_setup_ st
+
+
+[@ "substitute"]
+val keysetup:
+  st:state ->
+  k:uint8_p{length k = 32 /\ disjoint st k} ->
+  Stack unit
+    (requires (fun h -> live h st /\ live h k))
+    (ensures  (fun h0 _ h1 -> live h0 st /\ live h0 k /\ live h1 st /\ modifies_1 st h0 h1 /\
+      (let st0 = as_seq h0 st in let st1 = as_seq h1 st in let op_String_Access = Seq.index in
+       st1.[0] == st0.[0] /\
+       st1.[3] == st0.[3] /\
+       st1.[1] == Spec.Lib.uint32s_from_le 4 (Seq.slice (as_seq h0 k) 0 16) /\
+       st1.[2] == Spec.Lib.uint32s_from_le 4 (Seq.slice (as_seq h0 k) 16 32)
+       )))
+[@ "substitute"]
+let keysetup st k =
+  let k0 = vec_load128_le (Buffer.sub k 0ul 16ul) in
+  let k1 = vec_load128_le (Buffer.sub k 16ul 16ul) in
+  st.(1ul) <- k0;
+  st.(2ul) <- k1
+
+
+[@ "substitute"]
+val ctr_ivsetup:
+  st:state ->
+  ctr:U32.t ->
+  iv:uint8_p{length iv = 12 /\ disjoint st iv} ->
+  Stack unit
+    (requires (fun h -> live h st /\ live h iv))
+    (ensures  (fun h0 _ h1 -> live h1 st /\ modifies_1 st h0 h1 /\ live h0 iv /\ live h0 st /\
+      (let st0 = as_seq h0 st in let st1 = as_seq h1 st in let op_String_Access = Seq.index in
+       st1.[0] == st0.[0] /\
+       st1.[1] == st0.[1] /\
+       st1.[2] == st0.[2] /\
+       st1.[3] == Seq.cons ctr (Spec.Lib.uint32s_from_le 3 (as_seq h0 iv))) ))
+[@ "substitute"]
+let ctr_ivsetup st ctr iv =
+  let n0 = load32_le (Buffer.sub iv 0ul 4ul) in
+  let n1 = load32_le (Buffer.sub iv 4ul 4ul) in
+  let n2 = load32_le (Buffer.sub iv 8ul 4ul) in
+  let h = ST.get() in
+  assume (Seq.index (Spec.Lib.uint32s_from_le 3 (as_seq h iv)) 0 == n0);
+  assume (Seq.index (Spec.Lib.uint32s_from_le 3 (as_seq h iv)) 1 == n1);
+  assume (Seq.index (Spec.Lib.uint32s_from_le 3 (as_seq h iv)) 2 == n2);
+  let v =  vec_load_32x4 ctr n0 n1 n2 in
+  Seq.lemma_eq_intro (Seq.slice (vec_as_seq v) 1 4) (Spec.Lib.uint32s_from_le 3 (as_seq h iv));
+  Seq.lemma_eq_intro (vec_as_seq v) (Seq.cons ctr (Spec.Lib.uint32s_from_le 3 (as_seq h iv)));
+  st.(3ul) <- v
+
+
+[@ "c_inline"]
+val state_setup:
+  st:state ->
+  k:uint8_p{length k = 32 /\ disjoint st k} ->
+  n:uint8_p{length n = 12 /\ disjoint st n} ->
+  c:U32.t ->
+  Stack unit
+    (requires (fun h -> live h st /\ live h k /\ live h n))
+    (ensures (fun h0 _ h1 -> live h0 k /\ live h0 n /\ live h1 st /\ modifies_1 st h0 h1 /\
+      as_seq h1 st == Spec.Chacha20_vec.setup (as_seq h0 k) (as_seq h0 n) (U32.v c)))
+[@ "c_inline"]
+let state_setup st k n c =
+  let h0 = ST.get() in
+  constant_setup st;
+  keysetup st k;
+  ctr_ivsetup st c n;
+  let h = ST.get() in
+  Seq.lemma_eq_intro (as_seq h st) (Spec.Chacha20_vec.setup (as_seq h0 k) (as_seq h0 n) (U32.v c))
